Multisem/HeytingAlgebras.lean
@@ -1,0 +1,51 @@
+class HeytingAlgebra (P:Type u) where
+  top : P
+  bottom : P
+  conj : P -> P -> P
+  disj : P -> P -> P
+  impl : P -> P -> P
+class HeytingAlgebraLaws (P : Type u) extends HeytingAlgebra P where
+  conj_comm : ∀ x y, conj x y = conj y x
+  conj_assoc : ∀ x y z, conj (conj x y) z = conj x (conj y z)
+  disj_comm : ∀ x y, disj x y = disj y x
+  disj_assoc : ∀ x y z, disj (disj x y) z = disj x (disj y z)
+  distrib_left : ∀ x y z, conj x (disj y z) = disj (conj x y) (conj x z)
+  distrib_right : ∀ x y z, conj (disj x y) z = disj (conj x z) (conj y z)
+  -- TODO: missing impl laws
+
+class HeytingAlgebraMorphism (P : Type u)[HeytingAlgebra P](Q : Type v)[HeytingAlgebra Q] where
+  morph : P -> Q
+class HeytingAlgebraMorphismLaws (P : Type u)[HeytingAlgebra P](Q : Type v)[HeytingAlgebra Q] extends HeytingAlgebraMorphism P Q where
+  preserves_top : morph HeytingAlgebra.top = HeytingAlgebra.top
+  preserves_bottom : morph HeytingAlgebra.bottom = HeytingAlgebra.bottom
+  preserves_conj : ∀ x y, morph (HeytingAlgebra.conj x y) = HeytingAlgebra.conj (morph x) (morph y)
+  preserves_disj : ∀ x y, morph (HeytingAlgebra.disj x y) = HeytingAlgebra.disj (morph x) (morph y)
+  preserves_impl : ∀ x y, morph (HeytingAlgebra.impl x y) = HeytingAlgebra.impl (morph x) (morph y)
+
+
+instance pointwiseHA (X : Type v)(H : Type u)[HeytingAlgebra H] : HeytingAlgebra (X -> H) where
+  top := λ_ => HeytingAlgebra.top
+  bottom := λ_ => HeytingAlgebra.bottom
+  conj x y := λ p => HeytingAlgebra.conj (x p) (y p)
+  disj x y := λ p => HeytingAlgebra.disj (x p) (y p)
+  impl x y := λ p => HeytingAlgebra.impl (x p) (y p)
+
+instance pointwiseHALaws (X : Type v)(H : Type u)[HeytingAlgebraLaws H] : HeytingAlgebraLaws (X -> H) where
+  top := λ_ => HeytingAlgebra.top
+  bottom := λ_ => HeytingAlgebra.bottom
+  conj x y := λ p => HeytingAlgebra.conj (x p) (y p)
+  disj x y := λ p => HeytingAlgebra.disj (x p) (y p)
+  impl x y := λ p => HeytingAlgebra.impl (x p) (y p)
+  conj_comm x y := by { apply funext; intro p; apply HeytingAlgebraLaws.conj_comm }
+  conj_assoc x y z := by { apply funext; intro p; apply HeytingAlgebraLaws.conj_assoc }
+  disj_comm x y := by { apply funext; intro p; apply HeytingAlgebraLaws.disj_comm }
+  disj_assoc x y z := by { apply funext; intro p; apply HeytingAlgebraLaws.disj_assoc }
+  distrib_left x y z := by apply funext; intro p; apply HeytingAlgebraLaws.distrib_left
+  distrib_right x y z := by apply funext; intro p; apply HeytingAlgebraLaws.distrib_right
+
+instance PropHeyting : HeytingAlgebra Prop where
+  top := True
+  bottom := False
+  conj x y := x ∧ y
+  disj x y :=  x ∨ y
+  impl x y := x -> y
