Multisem/TemporalLogic.lean
@@ -1,0 +1,143 @@
+import Multisem.HeytingAlgebras
+
+def StateFormula (T : Type u) := T -> Prop
+
+instance StateFormulatHeyting (T : Type u): HeytingAlgebra (StateFormula T) := pointwiseHA T Prop
+
+namespace ltl
+  inductive LTLFormula (T : Type u) where
+    | true : LTLFormula T
+    | false : LTLFormula T
+    | stateProp : StateFormula T -> LTLFormula T
+    | not : LTLFormula T -> LTLFormula T
+    | next : LTLFormula T -> LTLFormula T
+    | or : LTLFormula T -> LTLFormula T -> LTLFormula T
+    -- "until" is a reserved keyword in Lean
+    | unt : LTLFormula T -> LTLFormula T -> LTLFormula T
+  -- Convenient shorthands for outside this namespace
+  def true {T : Type u} : LTLFormula T := LTLFormula.true
+  def false {T : Type u} : LTLFormula T := LTLFormula.false
+  def or {T : Type u} : LTLFormula T -> LTLFormula T -> LTLFormula T:= LTLFormula.or
+  def unt {T : Type u} : LTLFormula T -> LTLFormula T -> LTLFormula T:= LTLFormula.unt
+  def next {T : Type u} : LTLFormula T -> LTLFormula T:= LTLFormula.next
+  def not {T : Type u} : LTLFormula T -> LTLFormula T:= LTLFormula.not
+  
+  -- LTL is typically classical, so these are derived in the classic way
+  def and {T : Type u} (a b : LTLFormula T) : LTLFormula T :=
+    LTLFormula.not (LTLFormula.or (LTLFormula.not a) (LTLFormula.not b))
+  def impl {T : Type u} (a b : LTLFormula T) : LTLFormula T :=
+    LTLFormula.or (LTLFormula.not a) b
+  -- other derived forms
+  -- "finally" is a reserved keyword
+  def final {T : Type u} (a : LTLFormula T) : LTLFormula T :=
+    LTLFormula.unt LTLFormula.true a
+  -- TODO: G(lobally)
+  
+end ltl
+
+namespace ctlstar
+  mutual
+    inductive CTLStarFormula (T : Type u) where
+      | false
+      | true
+      | stateProp : StateFormula T -> CTLStarFormula T
+      | not : CTLStarFormula T -> CTLStarFormula T
+      | or : CTLStarFormula T -> CTLStarFormula T -> CTLStarFormula T
+      | A : CTLPathFormula T -> CTLStarFormula T
+      | E : CTLPathFormula T -> CTLStarFormula T
+    inductive CTLPathFormula (T : Type u) where
+      | starformula : CTLStarFormula T -> CTLPathFormula T
+      | not : CTLPathFormula T -> CTLPathFormula T
+      | or : CTLPathFormula T -> CTLPathFormula T -> CTLPathFormula T
+      | X : CTLPathFormula T -> CTLPathFormula T
+      | F : CTLPathFormula T -> CTLPathFormula T
+      | G : CTLPathFormula T -> CTLPathFormula T
+      | U : CTLPathFormula T -> CTLPathFormula T -> CTLPathFormula T
+    end
+
+  def and {T : Type u} (a b : CTLStarFormula T) : CTLStarFormula T :=
+    CTLStarFormula.not (CTLStarFormula.or (CTLStarFormula.not a) (CTLStarFormula.not b))
+  def impl {T : Type u} (a b : CTLStarFormula T) : CTLStarFormula T :=
+    CTLStarFormula.or (CTLStarFormula.not a) b
+
+end ctlstar
+
+namespace ctl
+  inductive CTLFormula (T : Type u) where
+    | false
+    | true
+    | stateProp : StateFormula T -> CTLFormula T
+    | not : CTLFormula T -> CTLFormula T
+    | or : CTLFormula T -> CTLFormula T -> CTLFormula T
+    | EG : CTLFormula T -> CTLFormula T
+    | EU : CTLFormula T -> CTLFormula T
+    | EX : CTLFormula T -> CTLFormula T
+    | AG : CTLFormula T -> CTLFormula T
+    | AU : CTLFormula T -> CTLFormula T
+    | AX : CTLFormula T -> CTLFormula T
+  def and {T : Type u} (a b : CTLFormula T) : CTLFormula T :=
+    CTLFormula.not (CTLFormula.or (CTLFormula.not a) (CTLFormula.not b))
+  def impl {T : Type u} (a b : CTLFormula T) : CTLFormula T :=
+    CTLFormula.or (CTLFormula.not a) b
+end ctl
+
+instance LTLHeyting (T : Type u) : HeytingAlgebra (ltl.LTLFormula T) where
+  top := ltl.true
+  bottom := ltl.false
+  conj := ltl.and
+  disj := ltl.or
+  impl := ltl.impl
+
+instance CTLHeyting (T : Type u) : HeytingAlgebra (ctl.CTLFormula T) where
+  top := ctl.CTLFormula.true
+  bottom := ctl.CTLFormula.false
+  disj := ctl.CTLFormula.or
+  conj := ctl.and
+  impl := ctl.impl
+
+instance CTLStarHeyting (T : Type u) : HeytingAlgebra (ctlstar.CTLStarFormula T) where
+  top := ctlstar.CTLStarFormula.true
+  bottom := ctlstar.CTLStarFormula.false
+  disj := ctlstar.CTLStarFormula.or
+  conj := ctlstar.and
+  impl := ctlstar.impl
+
+def ctl_to_ctlstar {T : Type u} (x : ctl.CTLFormula T) : ctlstar.CTLStarFormula T :=
+  match x with
+  | ctl.CTLFormula.false => ctlstar.CTLStarFormula.false
+  | ctl.CTLFormula.true => ctlstar.CTLStarFormula.true
+  | ctl.CTLFormula.or a b => ctlstar.CTLStarFormula.or (ctl_to_ctlstar a) (ctl_to_ctlstar b)
+  | ctl.CTLFormula.not a => ctlstar.CTLStarFormula.not (ctl_to_ctlstar a)
+  | ctl.CTLFormula.stateProp p => ctlstar.CTLStarFormula.stateProp p
+  | ctl.CTLFormula.AX a => ctlstar.CTLStarFormula.A (ctlstar.CTLPathFormula.X (ctlstar.CTLPathFormula.starformula (ctl_to_ctlstar a)))
+  | ctl.CTLFormula.AU a => ctlstar.CTLStarFormula.A (ctlstar.CTLPathFormula.U (ctlstar.CTLPathFormula.starformula ctlstar.CTLStarFormula.true) (ctlstar.CTLPathFormula.starformula (ctl_to_ctlstar a)))
+  | ctl.CTLFormula.AG a => ctlstar.CTLStarFormula.A (ctlstar.CTLPathFormula.G (ctlstar.CTLPathFormula.starformula (ctl_to_ctlstar a)))
+  | ctl.CTLFormula.EX a => ctlstar.CTLStarFormula.E (ctlstar.CTLPathFormula.X (ctlstar.CTLPathFormula.starformula (ctl_to_ctlstar a)))
+  | ctl.CTLFormula.EU a => ctlstar.CTLStarFormula.E (ctlstar.CTLPathFormula.U (ctlstar.CTLPathFormula.starformula ctlstar.CTLStarFormula.true) (ctlstar.CTLPathFormula.starformula (ctl_to_ctlstar a)))
+  | ctl.CTLFormula.EG a => ctlstar.CTLStarFormula.E (ctlstar.CTLPathFormula.G (ctlstar.CTLPathFormula.starformula (ctl_to_ctlstar a)))
+
+-- HA Morphisms
+
+-- CTL -> CTL*
+instance CTLStarMorphism (T : Type u) : HeytingAlgebraMorphism (ctl.CTLFormula T) (ctlstar.CTLStarFormula T) where
+  morph := ctl_to_ctlstar
+
+-- State formulas -> LTL & CTL
+instance ltl_state (T : Type u) : HeytingAlgebraMorphism (StateFormula T) (ltl.LTLFormula T) where
+  morph := ltl.LTLFormula.stateProp
+instance ctl_state (T : Type u) : HeytingAlgebraMorphism (StateFormula T) (ctl.CTLFormula T) where
+  morph := ctl.CTLFormula.stateProp
+
+-- State formulas -> CTL* by way of CTL
+instance ctl_star_state (T : Type u) : HeytingAlgebraMorphism (StateFormula T) (ctlstar.CTLStarFormula T) where
+  morph := HeytingAlgebraMorphism.morph ∘ (@HeytingAlgebraMorphism.morph (StateFormula T) (StateFormulatHeyting T) (ctl.CTLFormula T) (CTLHeyting T) (ctl_state T))
+
+
+-- Additional specs
+
+def ltlspec (T : Type u) (l:List String) [sem:Synth (ltl.LTLFormula T) l S] : (ltl.LTLFormula T) :=
+  sem.denotation
+def ctlspec (T : Type u) (l:List String) [sem:Synth (ctl.CTLFormula T) l S] : (ctl.CTLFormula T) :=
+  sem.denotation
+def ctlstarspec (T : Type u) (l:List String) [sem:Synth (ctlstar.CTLStarFormula T) l S] : (ctlstar.CTLStarFormula T) :=
+  sem.denotation
